feat: big advancement

Distributed/paper_proofs.lean
@@ -1,67 +1,11 @@
 -- Properties that check that the network is a valid network
-import Distributed.paper_implementation
+import Distributed.paper_model
+import Distributed.base_structures
 import Mathlib.Tactic.ByContra
 
 namespace Steps
+open PaperModel
 open Model
-
--- Init properties: Check that the program has a valid init state
-def coordinatorInits (c: Coordinator n) : Prop :=
-    c.decision = none ∧ c.yesVotes = emptySet ∧ c.noVotes = emptySet
-
-def participantInits (p: Participant n) (idx: Fin n): Prop :=
-    p.decision = none ∧ (p.hostid = idx)
-
-def networkInits (n: Network n): Prop :=
-    n.network = []
-
-def systemInits (s: System n) : Prop :=
-    networkInits s.network ∧ coordinatorInits s.coordinator ∧ ∀ i, participantInits (s.participants i) i
-
--- Steps: list all possible steps
-
-def ParticipantSendsPreference (p1: Participant n) (p2: Participant n) (snd: Message n) : Prop :=
-snd = Message.Vote p1.preference p1.hostid ∧ p2 = p1
-
-def CoordinatorReceivesPreference(c1: Coordinator n) (c2: Coordinator n) (rcv: Message n): Prop:= 
-    ∃ (pref: Model.Preference) (id: Fin n), rcv = Message.Vote pref id
-    ∧ if pref = Preference.Yes then
-      c2 = {c1 with yesVotes := insertElem c1.yesVotes id}
-    else
-      c2 = {c1 with noVotes := insertElem c1.noVotes id}    
-
-
-def CoordinatorMakesDecisionStep (c1: Coordinator n) (c2: Coordinator n) : Prop:=
-c1.decision = none ∧
-if count c1.yesVotes = n  then
-   c2 = {c1 with decision := some Decision.Commit}
-else if count c1.noVotes >= 1 then
-   c2 = {c1 with decision := some Decision.Abort}
-else
-   c2 = c1
-
-def CoordinatorSendDecideStep (c1: Coordinator n) (c2: Coordinator n) (m: Message n) : Prop:=
-∃ a, c1.decision = some a ∧ m = Message.Decide a
-
-def ParticipantReceiveDecisionStep (p1: Participant n) (p2: Participant n) (m: Message n) : Prop:=
-∃ a, m = Message.Decide a ∧ p1.decision = none ∧ p2 = {p1 with decision := some a}
-
-
-
-inductive step : System n -> System n -> Prop where
-| partSendPref: ∀ (s: System n) (i: Fin n) (p2: Participant n) (snd: Message n), ParticipantSendsPreference (s.participants i) p2 snd -> step s {s with participants := updateMap s.participants i p2, network := {s.network with network := snd :: s.network.network}}
-| coordRecvPref: ∀ (s: System n) (c2: Coordinator n) (rcv: Message n) , CoordinatorReceivesPreference s.coordinator c2 rcv -> rcv ∈ s.network.network-> step s {s with coordinator := c2, network := {s.network with network := s.network.network.erase rcv}}
-| coordMksDec: ∀ (s: System n) (c2: Coordinator n), CoordinatorMakesDecisionStep s.coordinator c2 -> step s {s with coordinator := c2}
-| coordSndDecStep: ∀ (s: System n) (snd: Message n), CoordinatorSendDecideStep s.coordinator s.coordinator snd -> step s {s with coordinator := s.coordinator, network := {s.network with network := snd :: s.network.network}}
-| partRecvDec: ∀ (s: System n) (p2: Participant n) (i: Fin n) (rcv: Message n), ParticipantReceiveDecisionStep (s.participants i) p2 rcv -> rcv ∈ s.network.network -> step s {s with participants := updateMap s.participants i p2, network := s.network}
-
-inductive steps : System n -> System n -> Prop where
-| refl : ∀ s1, steps s1 s1
-| trans: ∀ s1 s2 s3, steps s1 s2 -> step s2 s3 -> steps s1 s3 
-
-def validSystem (s: System n) :=
-∃ s0, systemInits s0  ∧ steps s0 s ∧ n ≠ 0
-
 
 theorem validSystemMapIds (s: System n) :
 validSystem s
@@ -75,11 +19,10 @@ validSystem s
    rename_i p i  m stepRule mInN ;simp [ParticipantReceiveDecisionStep] at stepRule; simp [updateMap]; grind
 
 
-
 theorem commitImpYesVotesIsNINV (s: System n) :
 validSystem s
 -> count s.coordinator.yesVotes ≠ n
--> (∀ i, (s.participants i).decision ≠  some Decision.Commit) ∧ Message.Decide Decision.Commit ∉ s.network.network ∧ s.coordinator.decision ≠ Decision.Commit := by
+-> (∀ i, (s.participants i).decision ≠ some Decision.Commit) ∧ Message.Decide Decision.Commit ∉ s.network.network ∧ s.coordinator.decision ≠ Decision.Commit := by
    intros validSys
    intro coordNeqN
    unfold validSystem at validSys; rcases  validSys with ⟨ s0, s0Inits, sSteps , nNeqZero⟩
