Distributed/base_structures.lean
@@ -1,0 +1,112 @@
+-- Structures useful to define our data structure
+namespace Model
+
+-- Definition of a Map Type
+def Map (n: Nat) (T: Type _) := (Fin n) -> T
+
+def updateMap (f: Map n T) (i: Fin n) (t: T): (Fin n) -> T:=
+    λ x => if i == x then t else f x
+
+-- Definition of a Set Type
+def Set (n: Nat) := Map n Bool
+
+@[simp]
+def emptySet : Set n:= λ _ => false
+
+@[simp]
+def fullSet: Set n := (λ _ => true)
+
+def insertElem (s: Set n) (i: Fin n) := updateMap s i true
+
+def contains (s: Set n) (i: Fin n): Bool := s i
+
+
+-- Function to count the number of elements inseide a Set
+def count_ (s: Set n) (i: Nat) (h: NeZero n): Nat :=
+  match i with
+  | 0 => 0
+  | a + 1 =>
+    if s (Fin.ofNat n a) then 1 + count_ s a h else  count_ s a h
+   
+
+def count (s: Set n): Nat :=
+  if h : (n ≠ 0) then
+     have : NeZero n := ⟨h⟩ 
+     count_ s n this
+  else
+        0
+
+
+
+
+-- Useful theorems for our implementations of Set and Map
+theorem fullSetImpN (s: Set n):
+count s = n
+-> n ≠ 0
+-> ∀ i, s i = true := by
+   induction n
+   . simp
+   . rename_i n IH
+     intros count_neq_one n_neq_zero
+     unfold count at *; simp at *
+     sorry
+     
+
+theorem setLimit (s: Set n):
+count s <= n := by
+      induction n
+      . unfold count count_; simp
+      . rename_i n IH
+        sorry
+        
+
+theorem insertIncreasesCount (s: Set n):
+count s <=  count (insertElem s i) := by
+sorry
+      
+      
+      
+    
+   
+theorem fullSetCannotIncrease (s: Set n):
+count s = n
+-> ∀ i, count (insertElem s i) = n := by
+   sorry
+
+
+theorem fullSetCannotIncreaseContra (s: Set n):
+∀ i, ¬(count (insertElem s i) = n)
+-> ¬count s = n:= by
+   have contr := fullSetCannotIncrease s; grind
+
+
+
+theorem fullSetCountsN (n: Nat):
+count (@fullSet n) = n := by
+  unfold fullSet count count_
+  induction n
+  . grind
+  . rename_i n IH
+    simp at *; split at IH; rw [<-IH]; simp [count_]
+    split at IH; simp [count_]
+    rename_i i a aNeq; simp [count_]
+    sorry
+
+
+
+theorem countSupImpContains (i: Nat) (s: Set a) :
+0 < i
+-> i < count s
+-> ∃ j, contains s j == true := by sorry
+
+
+
+def setMaxContainsBoth (set1 set2: Set a):
+count set1 > a / 2
+-> count set2 > a / 2
+-> ∃ i, contains set1 i ∧ contains set2 i := by
+   intros countSet1 countSet2
+   induction a
+   sorry
+   sorry
+           
