Distributed/old_imp/paxos_proof_new.lean
@@ -1,0 +1,65 @@
+import Distributed.base_structures
+import Distributed.paxos_model
+import Mathlib.Tactic.ByContra
+
+open Model
+open PaxosModel
+namespace PaxosProof
+
+
+@[simp]
+def learner_invariant (learner: Learner a l) (v: Value) :=
+(∃ (s: Set a), count s > a / 2 ∧ (∀ i, contains s i -> learner.decMap i = v ))
+
+
+
+theorem unique_set (learners: Map l (Learner a l)) (v1 v2: Value) (j: Fin l):
+(∃ s, a / 2 < count s ∧ ∀ (i : Fin a), contains s i = true → (learners j).decMap i = some v1)
+-> (∃ s, a / 2 < count s ∧ ∀ (i : Fin a), contains s i = true → (learners j).decMap i = some v2)
+-> v1 = v2 := by sorry
+
+theorem valid_sys_imp_sing_val_contra (s: System a l p):
+systemIsValid s
+-> ∃ v, ∀ j, (s.learners j).decide ≠ none
+→ (s.learners j).decide = some v ∧ learner_invariant (s.learners j) v  := by
+  intros sIsValid; simp [systemIsValid] at sIsValid; rcases sIsValid with ⟨ s0, s0Inits, s0Steps⟩
+  induction s0Steps with
+  | refl =>
+    exists 1;
+    simp [systemInits, networkInits, proposerInits, acceptorInits, learnerInits] at s0Inits
+    simp [s0Inits]
+  | trans s1 s2 s0Steps s1Step IH =>
+    cases s1Step with
+    | failureStep stepRule => cases stepRule; simp; sorry
+    | workingStep stepRule =>
+      cases stepRule with
+      | choosefinalvalue l1 v' i stepRule =>
+        rcases IH with ⟨v, IHProp⟩
+        exists v; intros j learnerUpd; simp [updateMap] at *
+        split <;> try grind
+        
+          
+
+          
+          
+
+
+theorem valid_sys_imp_sing_val (s : System a l p):
+systemIsValid s
+-> ∃ v, ∀ j, (s.learners j).decide = some v ∨ (s.learners j).decide = none:= by
+   intros sIsValid
+   have cc := valid_sys_imp_sing_val_contra s sIsValid
+   rcases cc with ⟨v, exec ⟩; exists v
+   grind
+   
+
+theorem learners_choice_is_unique (s : System a l p):
+ ∀ i j v1 v2, systemIsValid s -> (s.learners i).decide = some v1 -> (s.learners j).decide = some v2 -> v1 = v2 := by
+   intro i j v1 v2 sIsValid sDecV1 sDecV2
+   have t1 := valid_sys_imp_sing_val s
+   grind
+     
+   
+   
+   
+   
