Distributed/old_imp/paxos_proof_new2.lean
@@ -1,0 +1,193 @@
+import Distributed.base_structures
+import Distributed.paxos_model
+import Mathlib.Tactic.ByContra
+
+open Model
+open PaxosModel
+namespace PaxosProof
+
+@[simp]
+def learner_invariant (s1: System a l p) (learner: Learner a l) (n: Network) (v: Value) :=
+(∃  (s: Set a), count s > a / 2 ∧  (∀ i, contains s i -> learner.decMap i = v ∨ (@Message.Learn a (i, v) ∈  n.messages) ∨ (∃ id, (s1.acceptors i).accepted = some (id, v)))) 
+
+
+def acceptorsAreEnoughOfValue (accs:  Map a (Acceptor a)) (v: Value) :=
+(∃ (s1: Set a), count s1 > a / 2 ∧  (∀ (i : Fin a), contains s1 i = true ->  (∀ k, (accs i).accepted = some (v, k))))
+
+/--
+def lemma1 (s: System a l p) (v: Value):
+systemIsValid s
+->  acceptorsAreEnoughOfValue s.acceptors v
+-> ∀ j v1, (s.learners j).decide = some v1
+-> v1 = v := by sorry
+--/
+
+
+
+
+-- HELPER LEMMAS
+
+def lemma31 (s: System a l p) (v1 v2: Value) (j: Fin l):
+learner_invariant s (s.learners j) s.network v1
+-> learner_invariant s (s.learners j) s.network v2
+-> v1 = v2 := by
+   intros acc1 acc2
+   unfold learner_invariant at *; simp at *
+   rcases acc1 with ⟨ set1, countSet1, set1Prop⟩
+   rcases acc2 with ⟨ set2, countSet2, set2Prop⟩
+   have finalC := setMaxContainsBoth set1 set2 countSet1 countSet2
+   rcases finalC with ⟨ i, ⟨ set1Contains, set2Contains ⟩ ⟩
+   have set2C := set2Prop i set2Contains ; have set1C := set1Prop i set1Contains; clear set2Prop set1Prop
+   sorry
+   
+
+def lemma3 (s: System a l p) (v1 v2: Value):
+systemIsValid s
+-> acceptorsAreEnoughOfValue s.acceptors v1
+-> acceptorsAreEnoughOfValue s.acceptors v2
+-> v1 = v2 := by
+   intros sIsValid acc1 acc2
+   unfold acceptorsAreEnoughOfValue at *
+   rcases acc1 with ⟨ set1, countSet1, set1Prop⟩
+   rcases acc2 with ⟨ set2, countSet2, set2Prop⟩
+   have finalC := setMaxContainsBoth set1 set2 countSet1 countSet2
+   rcases finalC with ⟨ i, ⟨ set1Contains, set2Contains ⟩ ⟩
+   have set2C := set2Prop i; have _ := (set2C set2Contains 0) 
+   have set1C := set1Prop i ; have _ := (set1C set1Contains 0)
+   grind
+
+-- MAIN INVARIANT
+def accept_inv (s1 s2: System a l p) (v: Value):
+step s1 s2
+-> (acceptorsAreEnoughOfValue s1.acceptors v)
+-> (acceptorsAreEnoughOfValue s2.acceptors v) := by
+   sorry
+
+
+def lemma0 (s1 s2: System a l p) (v: Value):
+step s1 s2
+-> ¬ (acceptorsAreEnoughOfValue s2.acceptors v)
+-> ¬ (acceptorsAreEnoughOfValue s1.acceptors v) := by
+   intros s1Step notEnoughAcc
+   have contra := accept_inv s1 s2 v s1Step
+   grind
+
+     
+
+def lemma1 (s1 s2: System a l p) (v: Value):
+step s1 s2
+-> ¬ (acceptorsAreEnoughOfValue s2.acceptors v)
+-> ∀ j, (s1.learners j).decide = none
+-> (∀ v', ¬ (learner_invariant s1 (s1.learners j) s1.network v'))
+-> (s2.learners j).decide = none ∧ (∀ v', ¬ (learner_invariant s2 (s2.learners j) s2.network v')):= by
+   intros stepCase acceptorOfEnoughValu s1DecNone decNone learnInv
+   cases stepCase with
+   | failureStep stepRule =>
+     cases stepRule with
+     | lostmessage  m n1 stepRule =>
+       constructor <;> try grind
+       simp at *; intros v'' x xCounts
+       sorry
+   | workingStep stepRule =>
+     cases stepRule with
+     | receivelearner i l2 mess v' j stepRule =>
+       rcases stepRule with ⟨messNat, messInN, learnIsNone, l2Nat ⟩
+       constructor
+       . simp [updateMap]; split <;> try grind
+         sorry
+       . subst_vars; simp at *
+         intros v'' set1 countSet1
+         have ⟨ x, xContains, xDecIsNone, messNotInN ⟩:= learnInv v'' set1 countSet1
+         exists x; simp [xContains, messNotInN];
+         simp [updateMap]; split <;> try grind
+         sorry
+     | choosefinalvalue l2 v' i stepRule =>
+       simp at *
+       rcases stepRule with ⟨s, countS, sNat, s1DecNone, l2Nat ⟩
+       constructor <;> try grind
+       . simp [updateMap]; split <;> try grind
+         subst_vars; simp
+         have cc := lemma31 s1 v' v i; simp at cc
+         have ⟨x, xContains, xNat ⟩  := (learnInv v') s countS
+         have res := sNat x xContains; simp [res] at xNat
+       . intros v'' set1 countSet1
+         have ⟨ x, xContains, xSome ⟩  := learnInv v'' set1 countSet1
+         exists x; simp [updateMap]; split <;> try grind
+      | sendlearner => sorry
+      | receiveacceptor id i j  v'' acc mess stepRule =>
+        simp at *
+        rcases stepRule with ⟨mNat, accNat ⟩
+        subst_vars
+        constructor <;> try grind
+        intros v'' x xCounts
+        have ⟨set1, xTrue, xDecMapFails, xInMess, xNotSome ⟩ := learnInv v'' x xCounts
+        
+      | sendacceptor v'  v'' n2 i stepRule =>
+        simp at *
+        rcases stepRule with ⟨mNat, accNat ⟩
+        subst_vars
+        constructor <;> try grind
+        intros v'' x xCounts
+        have ⟨set1, xTrue, xDecMapFails, xInMess, xNotSome ⟩ := learnInv v'' x xCounts
+        grind
+      | receivepromise i c maxN accId maxV prop mess stepRule=>
+        simp at *
+        rcases stepRule with ⟨mNat, accNat ⟩
+        subst_vars
+        constructor <;> try grind
+        intros v'' x xCounts
+        have ⟨set1, xTrue, xDecMapFails, xInMess, xNotSome ⟩ := learnInv v'' x xCounts
+        grind
+      | sendpromise _  i pid m acc n stepRule =>
+        simp at *
+        rcases stepRule with ⟨mNat, accNat ⟩
+        subst_vars
+        constructor <;> try grind
+        intros v'' x xCounts
+        have ⟨set1, xTrue, xDecMapFails, xInMess, xNotSome ⟩ := learnInv v'' x xCounts
+        grind
+      | sendprepare n2 n1 m i prop  stepRule =>
+        simp at *
+        rcases stepRule with ⟨mPrep, addMessInNet, propNat ⟩
+        subst_vars
+        constructor <;> try grind
+        intros v'' x xCounts
+        have ⟨set1, xTrue, xDecMapFails, xInMess, xNotSome ⟩ := learnInv v'' x xCounts
+        grind
+
+def lemma2 (s: System a l p) (v: Value):
+systemIsValid s
+->  ¬ (acceptorsAreEnoughOfValue s.acceptors v)
+-> ∀ j, (s.learners j).decide = none ∧ (∀ v', ¬ (learner_invariant s (s.learners j) s.network v')):= by
+   intros sIsValid notEnoughAcceptors j
+   simp [systemIsValid] at sIsValid; rcases sIsValid with ⟨ s0, s0Inits, s0Steps⟩
+   induction s0Steps with
+   | refl =>
+     unfold systemInits learnerInits at s0Inits; simp [s0Inits]
+     intros x countX; cases a <;> try grind
+     sorry
+   | trans s1 s2 s0Steps s1Step IH =>
+     have l1 := lemma1 s1 s2 v
+     have l2 := lemma0 s1 s2     
+     grind
+     
+   
+   
+
+
+
+
+theorem learners_choice_is_unique (s : System a l p):
+ ∀ i j v1 v2, systemIsValid s -> (s.learners i).decide = some v1 -> (s.learners j).decide = some v2 -> v1 = v2 := by
+   intro i j v1 v2 sIsValid sDecV1 sDecV2
+   by_cases c1:(acceptorsAreEnoughOfValue s.acceptors v1)
+   . by_cases c2:(acceptorsAreEnoughOfValue s.acceptors v2)
+     . have eqVal := lemma3 s v1 v2 sIsValid c1 c2; exact eqVal
+     . have contra := lemma2 s v2 sIsValid c2; simp [contra] at sDecV2 
+   . have contra := lemma2 s v1 sIsValid c1; simp [contra] at sDecV1
+  
+     
+   
+   
+   
+   
