Distributed/old_imp/paxos_proof_old.lean
@@ -1,0 +1,140 @@
+import Distributed.base_structures
+import Distributed.paxos_model
+import Mathlib.Tactic.ByContra
+
+open Model
+open PaxosModel
+namespace PaxosProof
+
+
+theorem learner_choice_is_constant_inv_step (s s': System a l p):
+ ∀ i v, (s.learners i).decide = some v -> step s s' -> (s'.learners i).decide = some v := by
+   intros i v v_decides s_step_s' 
+   cases s_step_s' with
+   | workingStep =>
+     rename_i curr_step
+     cases curr_step <;> try grind
+     simp at *
+     rename_i i_ l2 m v_ netState
+     rcases netState with ⟨mNat, sLearn, sDec, l2Val⟩
+     rcases l2 with ⟨lLeq, vVal⟩
+     sorry
+     sorry
+     sorry
+     sorry
+     sorry
+     sorry
+   | failureStep =>
+     rename_i curr_step
+     cases curr_step <;> try grind
+     
+     
+
+theorem learner_choice_is_constant_inv (s s': System a l p):
+ ∀ i v, (s.learners i).decide = some v -> steps s s' -> (s'.learners i).decide = some v := by
+   intros i v sDecV sSteps
+   induction sSteps
+   . assumption
+   . rename_i s1 s2 _ _ IH
+     apply (learner_choice_is_constant_inv_step s1 s2 i v IH)
+     assumption
+     
+
+theorem learner_choice_is_constant (s s': System a l p):
+ ∀ i v, (s.learners i).decide = some v -> steps s s' -> (s'.learners i).decide = some v := by
+   apply learner_choice_is_constant_inv
+
+    
+theorem acceptor_choice_is_constant_inv_step (s s': System a l p):
+ ∀ i v, (s.acceptors i).accepted = some v -> step s s' -> (s'.acceptors i).accepted = some v := by
+   intros i v v_decides s_step_s' 
+   cases s_step_s' with
+   | workingStep =>
+     rename_i curr_step
+     cases curr_step <;> try grind
+     simp at *
+     rename_i pid i_ l2 acc m currState
+     rcases currState with ⟨mAcc, sAccPid, sAccNone, accVal ⟩ 
+     by_cases (i = i_)
+     . sorry
+     . unfold updateMap
+       grind
+   | failureStep =>
+     rename_i curr_step
+     cases curr_step <;> try grind
+     
+     
+
+theorem acceptor_choice_is_constant_inv (s s': System a l p):
+ ∀ i v, (s.acceptors i).accepted = some v -> steps s s' -> (s'.acceptors i).accepted = some v := by
+   intros i v sDecV sSteps
+   induction sSteps
+   . assumption
+   . rename_i s1 s2 _ _ IH
+     apply (acceptor_choice_is_constant_inv_step s1 s2 i v IH)
+     assumption
+     
+
+theorem acceptor_choice_is_constant (s s': System a l p):
+ ∀ i v, (s.acceptors i).accepted = some v -> steps s s' -> (s'.acceptors i).accepted = some v := by
+   apply acceptor_choice_is_constant_inv
+
+
+@[simp]
+def learner_invariant (ls: Map l (Learner a l)) (v1 v2: Value):=
+(∀ j v (s1: Set a), count s1 > a / 2 -> (∀ (i : Fin a), contains s1 i = true → (ls j).decMap i = v) )
+∧ ∀ i j, ((ls j).decide ≠ some v2 ∨  (ls i).decide ≠ some v1)
+
+
+theorem learners_choice_is_unique_inv (s: System a l p):
+∀ v1 v2, systemIsValid s-> v1 ≠ v2 -> learner_invariant s.learners v1 v2
+:= by
+  intros v1 v2 sIsValid v1NeqV2
+  unfold systemIsValid at sIsValid; rcases sIsValid with ⟨s0, sInits, sSteps ⟩
+  induction sSteps with
+  | refl =>
+    simp [systemInits, learnerInits, acceptorInits, networkInits, proposerInits] at sInits
+    simp [sInits] 
+  | trans s1 s2 s0_steps_s1 s1_step_s2 IH =>
+    cases s1_step_s2 with
+    | failureStep stepRule =>
+      cases stepRule <;> try grind
+    | workingStep stepRule =>
+      cases stepRule with
+      | sendprepare =>
+        grind
+      | sendpromise => grind
+      | receivepromise => grind
+      | sendacceptor => grind
+      | receiveacceptor => grind
+      | sendlearner => grind
+      | receivelearner  i k l2 m v id stepRule =>
+        simp [updateMap]
+        simp at stepRule; rcases stepRule with ⟨ mNat, decNat, l2Nat⟩
+        subst_vars
+        sorry
+      | choosefinalvalue  l2 v k stepRule =>
+        simp [updateMap] at *
+        rcases stepRule with ⟨set1, s1Bound, s1Nat, l2Nat⟩
+        rcases IH with ⟨ ⟨ v', leftRule⟩ , rightRule ⟩ 
+        constructor
+        . exists v'; subst l2Nat
+          intros i st1 st1Bound j stNat 
+          sorry
+        . intros i j; split <;> split <;> try grind
+          cases rightRule i j <;> try grind
+          subst_vars; simp; left
+          
+          
+        
+        
+        
+theorem learners_choice_is_unique (s : System a l p):
+ ∀ i j v1 v2,systemIsValid s -> (s.learners i).decide = some v1 -> (s.learners j).decide = some v2 -> v1 = v2 := by
+   intros i j v1 v2
+   have cc := learners_choice_is_unique_inv s v1 v2
+   simp at cc
+   by_contra contra
+   grind
+   
+   
