Distributed/paxos_model.lean
@@ -1,0 +1,165 @@
+-- Base model for the paxos consensus algorithm
+import Distributed.base_structures
+namespace PaxosModel
+open Model
+
+-- Type to represent the values chosen by the algorithm
+def Value := Nat
+deriving OfNat, BEq, DecidableEq, Ord, LT
+
+-- Type to represent the Id for the proposals issued by the proposers
+
+def PropId := Nat
+deriving OfNat, BEq, DecidableEq, Ord, LT, HAdd, HMul, HMod, LE
+
+-- Type to represent the messages sent by the values
+inductive Message where
+| Prepare (propId: PropId) : Message
+| Promise (propId: PropId) (acceptId: Nat) (propVal: (Option Value) × PropId): Message
+| Accept (a: PropId × Value): Message
+| Learn (v: Fin a × Value × PropId )
+
+
+structure Proposer (p a: Nat) where
+id: Fin p
+propVal: Option Value
+propId: PropId
+accPropId: PropId
+propRec: Set a
+
+def uniqueId (prop: Proposer p a): PropId :=
+    (prop.propId * p + prop.id.toNat)
+
+structure Acceptor (a: Nat) where
+id: Fin a
+maxPrepareId: PropId
+maxProp: Option Value
+accepted: Option (Value × PropId)
+
+
+structure Learner (a: Nat) (l: Nat) where
+id: Fin l
+decMap: (Fin a) -> Option (Value × PropId)
+decide: Option Value
+
+structure Network where
+messages: List (Message)
+
+structure System (a: Nat) (l: Nat) (p: Nat) where
+learners: Map l (Learner a l)
+acceptors: Map a (Acceptor a)
+proposers: Map p (Proposer p a)
+network: Network
+
+
+-- Failure steps
+@[simp]
+-- Case if the message dissapears from the network
+def MessageIsLost (m: Message) (n1: Network) (n2: Network): Prop :=
+    n1.messages = m :: n2.messages  
+
+
+-- In this case we do not add the possibility of a duplicate step since it is already covered by the base model (since messages are not deleted at reception they can be read multiple times by multiple endpoints)
+inductive FailureStep: System a l p -> System a l p -> Prop where
+| lostmessage : ∀ (s1: System a l p) m n2, MessageIsLost m s1.network n2
+-> FailureStep s1 {s1 with network := n2}
+
+
+
+
+
+-- Algorithm steps
+@[simp]
+-- A proposer sends a proposal in the network with a new Id
+def ProposerSendsPrepare  (p1 p2: Proposer p a) (n1 n2: Network) (m: Message) := 
+m = Message.Prepare (uniqueId p1)  ∧ n2.messages = m :: n1.messages ∧ p2 = {p1 with propId := uniqueId p1, propVal := none, propRec := emptySet, accPropId := 0 }
+
+@[simp]
+def AcceptorReceivesPrepare (n: PropId) (a1 a2: Acceptor a) (n1 n2: Network) (m: Message) :=
+   (m ∈ n1.messages ∧ m = Message.Prepare n ∧ n > a1.maxPrepareId) ∧ a2 = {a1 with maxPrepareId := n} ∧ n2.messages = (Message.Promise n a1.id (a1.maxProp, a1.maxPrepareId)) :: n1.messages
+
+@[simp]
+def ProposerReceivesPromise (maxP: Nat) (accId: Fin a) (maxV: Option Value) (p1 p2: Proposer p a) (n: Network) (m: Message) :=
+    m = Message.Promise p1.propId accId (maxV, maxP) ∧  m ∈ n.messages ∧ 
+    if (maxP > p1.accPropId && maxV != none)
+    then  p2 = {p1 with propRec := insertElem p1.propRec accId, accPropId := maxP, propVal := maxV}
+    else p2 = {p1 with propRec := insertElem p1.propRec accId}
+
+@[simp]
+def ProposerSendsAcceptor (v: Value) (p: Proposer p a) (n1 n2: Network) :=
+    count p.propRec > (a / 2) ∧
+    if p.propVal == some v then
+       n2.messages = (Message.Accept (p.propId, v)) :: n1.messages
+    else
+       n2.messages = (Message.Accept (p.propId, v)) :: n1.messages 
+    
+@[simp]
+def AcceptorAccepts (id: PropId) (v: Value) (a1 a2: Acceptor a) (m: Message) :=
+    m = Message.Accept (id, v) ∧ a1.maxPrepareId < id 
+    ∧ a2 = {a1 with accepted := some (id, v)}
+
+@[simp]
+def SendLearner (acc: Acceptor a) (n1 n2: Network) (v: Value) (id: PropId) :=
+    acc.accepted = some (id, v) ∧ 
+    n2.messages = (Message.Learn (acc.id, v, id)) :: n1.messages
+
+@[simp]
+def RecvLearner (n: Network) (l1 l2: Learner a l) (m: Message) (v: Value) (acc: Fin a) (id: PropId):=
+    m = Message.Learn (acc, v, id) ∧ m ∈ n.messages ∧ l1.decide = none ∧
+    l2 = {l1 with decMap := updateMap l1.decMap acc (some (v, id))} 
+
+@[simp]
+def ChooseVal (l1 l2: Learner a l) (v: Value) (id: PropId):=
+    ∃ (s: Set a), count s > a / 2 ∧ (∀ i, contains s i -> l1.decMap i = (v, id))
+    ∧ l1.decide = none ∧  l2 = {l1 with decide := some v}
+
+
+inductive WorkingStep {a l p: Nat}: System a l p -> System a l p -> Prop where
+| sendprepare: ∀ s n2 m i p2, ProposerSendsPrepare (s.proposers i) p2 s.network n2 m -> WorkingStep s {s with proposers := updateMap s.proposers i p2, network := n2}
+| sendpromise: ∀ s i n m a2 n2, AcceptorReceivesPrepare n (s.acceptors i) a2 s.network n2 m -> WorkingStep s {s with network := n2}
+| receivepromise: ∀ i s maxN accId maxV p2 m, ProposerReceivesPromise maxN accId maxV (s.proposers i) p2 s.network m -> WorkingStep s {s with proposers := updateMap s.proposers i p2}
+| sendacceptor : ∀ s v n2 i, ProposerSendsAcceptor v (s.proposers i) s.network n2 -> WorkingStep s {s with network := n2}
+| receiveacceptor: ∀ id s i v a2 m, AcceptorAccepts id v (s.acceptors i) a2 m -> WorkingStep s {s with acceptors := updateMap s.acceptors i a2}
+| sendlearner: ∀ s i n2 v id, SendLearner (s.acceptors i) s.network n2 v id -> WorkingStep s {s with network := n2}
+| receivelearner: ∀ s i l2 m v id acc, RecvLearner (s.network) (s.learners i) l2 m v acc id -> WorkingStep s {s with learners := updateMap s.learners i l2}
+| choosefinalvalue: ∀ l2 v i id, ChooseVal (s.learners i) l2 v id -> WorkingStep s  {s with learners := updateMap s.learners i l2}
+-- All possible steps merged
+inductive step: System a l p -> System a l p -> Prop where
+| workingStep : ∀ s1 s2, WorkingStep s1 s2 -> step s1 s2
+--| failureStep: ∀ s1 s2, FailureStep s1 s2 -> step s1 s2
+-- TODO: I commented the failure step t work with it, maybe revert later
+
+inductive steps : System a l p -> System a l p -> Prop where
+| refl : ∀ s1, steps s1 s1
+| trans: ∀ s1 s2 s3, steps s1 s2 -> step s2 s3 -> steps s1 s3
+
+
+def networkInits (n_ : Network) :=
+    n_.messages = []
+
+
+def proposerInits (p_: Proposer p a) (i: Fin p) :=
+    p_.id = i ∧ p_.propVal = none ∧ p_.propId = p_.id.toNat ∧ p_.accPropId = 0 ∧ p_.propRec = emptySet
+
+
+def acceptorInits (a_: Acceptor a) (i: Fin a) :=
+    a_.id = i ∧ a_.maxPrepareId = 0 ∧ a_.maxProp = none ∧ a_.accepted = none
+
+
+def learnerInits (l_: Learner a l) (i: Fin l) :=
+    l_.id = i ∧ l_.decide = none ∧ l_.decMap = (λ _ => none)
+
+
+-- Definition of a system that initiates well
+def systemInits (s: System a l p) :=
+   networkInits s.network
+   ∧ (∀ i, proposerInits (s.proposers i) i)
+   ∧ (∀ j, acceptorInits (s.acceptors j) j)
+   ∧ (∀ k, learnerInits (s.learners k) k)
+   ∧ (a >= 2 ∧ l > 0 ∧ p > 0)
+
+
+def systemIsValid (s: System a l p) :=
+    ∃ s0, systemInits s0 ∧ steps s0 s
+
+
