Distributed/paxos_proof.lean
@@ -1,0 +1,109 @@
+import Distributed.base_structures
+import Distributed.paxos_model
+import Mathlib.Tactic.ByContra
+
+open Model
+open PaxosModel
+namespace PaxosProof
+
+
+@[simp]
+def set_invariant (s1: System a l p) (v: Value) (learnerId: Fin l) :=
+(∃  (s: Set a), count s > a / 2 ∧  (∀ i, contains s i -> (s1.learners learnerId).decide = some v ∨ (s1.learners learnerId).decMap i = v ∨ (@Message.Learn a (i, v) ∈ s1.network.messages) ∨ (∃ id, (s1.acceptors i).accepted = some (id, v)))) 
+
+
+/--
+def setCounts (s: System a l p) (v1 v2: Value) (j: Fin l):
+set_invariant s v1 j
+-> set_invariant s v2 j
+-> v1 = v2 := by
+   sorry
+
+
+
+
+theorem inv2_prop (s1 s2: System a l p) (j: Fin l):
+step s1 s2
+-> ((s1.learners j).decide = none ∧ ∀ (v' : Value), ¬set_invariant s1 v' j)
+-> (s2.learners j).decide = none ∧ ∀ (v' : Value), ¬set_invariant s2 v' j := by
+   intros s1Step IH
+   simp [set_invariant] at *
+   cases s1Step with
+   | failureStep stepRule =>
+     cases stepRule with
+     | lostmessage m n2 stepRule =>
+       simp at *; simp [IH]
+       intros v' set countSet
+       rcases (IH.right v' set countSet) with ⟨ x, setContains, decInside, decMap, messIn, acceptedOk ⟩ ; clear IH
+       grind
+   | workingStep stepRule =>
+     cases stepRule with
+     | choosefinalvalue l2 v i stepRule =>
+       simp at *;simp [updateMap]; split <;> try grind
+       rename_i eq; subst eq
+       rcases stepRule with ⟨set1, set1Count, set1Contains,set1None, l2Nat ⟩
+       subst l2Nat; exfalso;
+       rcases (IH.right v set1 set1Count) with ⟨ x, setContains, decInside, decMap, messIn, acceptedOk ⟩ ; clear IH
+       grind
+     | _ => sorry
+       
+--/
+
+
+theorem inv_proof (s1 s2: System a l p) (v: Value):
+step s1 s2
+-> ∀ j, (s2.learners j).decide ≠ some v
+-> (s1.learners j).decide ≠ some v  := by
+   intros s1Step j IH
+   by_contra contra
+   cases s1Step <;> rename_i stepRule <;> cases stepRule <;> try grind
+   . rename_i i learn m v' x stepRule; simp at *
+     have ⟨ learnNat,mInNet, learnDec, iNat ⟩ := stepRule;clear stepRule; subst_vars
+     unfold updateMap at IH; split at IH <;> try grind
+   . rename_i l2 v' u stepRule; simp at *
+     have ⟨set, setCount, setContains, l1None, l2Nat ⟩ := stepRule; clear stepRule
+     subst l2Nat; simp [updateMap] at IH; split at IH <;> try grind
+
+theorem valid_sys_imp_sing_val_contra (s: System a l p):
+systemIsValid s
+-> ∃ v, ∀ j, (s.learners j).decide ≠ some v
+→ (s.learners j).decide = none ∧ (∀ v', ¬ set_invariant s v' j) := by
+  intros sIsValid;
+  simp [systemIsValid] at sIsValid
+  have ⟨ s0, s0Inits, s0Steps ⟩ := sIsValid; clear sIsValid
+  induction s0Steps with
+  | refl =>
+    simp [systemInits, learnerInits, networkInits, acceptorInits] at s0Inits
+    exists 1; simp [s0Inits]
+    intros j v' set1 setCount
+    have cc := countSupImpContains (a / 2) set1; simp [s0Inits] at cc
+    have cc_ := cc setCount; exact cc_
+  | trans s1 s2 s0Steps s1Step IH=>
+    rcases IH with ⟨ v, IHApp ⟩
+    exists v; intros j s2DecidesNone
+    have inv_app := inv_proof s1 s2 v s1Step j s2DecidesNone
+    have IHProp := IHApp j inv_app
+    have ind_proof := inv2_prop s1 s2 j s1Step IHProp
+    grind
+  
+     
+   theorem valid_sys_imp_sing_val (s : System a l p):
+systemIsValid s
+-> ∃ v, ∀ j, (s.learners j).decide = some v ∨ (s.learners j).decide = none:= by
+   intros sIsValid
+   have cc := valid_sys_imp_sing_val_contra s sIsValid
+   rcases cc with ⟨v, exec ⟩; exists v
+   grind
+   
+
+theorem learners_choice_is_unique (s : System a l p):
+ ∀ i j v1 v2, systemIsValid s -> (s.learners i).decide = some v1 -> (s.learners j).decide = some v2 -> v1 = v2 := by
+   intro i j v1 v2 sIsValid sDecV1 sDecV2
+   have t1 := valid_sys_imp_sing_val s
+   grind
+     
+   
+
+   
+   
+   
