Distributed/paxos_proof3.lean
@@ -1,0 +1,65 @@
+import Distributed.base_structures
+import Distributed.paxos_model
+import Mathlib.Tactic.ByContra
+
+open Model
+open PaxosModel
+namespace PaxosProof
+
+
+@[simp]
+def set_invariant (s1: System a l p) (v: Value) (learnerId: Fin l) :=
+(∃  (s: Set a), count s > a / 2 ∧  (∀ i, contains s i -> ((s1.learners learnerId).decMap i = v ∧ (s1.learners learnerId).decide = some v ∧  (∃ id, (s1.acceptors i).accepted = some (id, v))))) 
+
+
+
+   
+
+
+
+
+theorem decide_imp_set_exists (s: System a l p) (j: Fin l) (v: Value):
+systemIsValid s
+-> (s.learners j).decide = some v
+-> set_invariant s v j := by
+   intros sIsValid learnIsSome
+   simp [systemIsValid] at sIsValid
+   --have absCase := absCase s j v
+   rcases sIsValid with ⟨ s0, s0Inits, s0Steps⟩
+   induction s0Steps with
+   | refl =>
+     simp [systemInits, learnerInits] at s0Inits
+     simp [s0Inits] at learnIsSome
+   | trans s1 s2 s0Steps s1Step IH=>
+     cases s1Step with
+     | failureStep stepRule=>
+       cases stepRule; rename_i m n2 stepRule; 
+       simp at stepRule ⊢ learnIsSome; have IHApp := IH learnIsSome; simp at IHApp; rcases IHApp with ⟨ set, setCount, setContains ⟩
+       exists set;
+     | workingStep stepRule =>
+       cases stepRule with
+       | choosefinalvalue learner v' i stepRule=>
+         simp at *
+
+theorem set_inv_is_unique (s: System a l p) (v1 v2: Value) (i j: Fin l):
+a >=  2
+-> set_invariant s v1 i
+-> set_invariant s v2 j
+-> v1 = v2 := by
+   intros aBound inv1 inv2
+   simp at inv1 inv2
+   rcases inv1 with ⟨ set1, countSet1, containsSet1⟩
+   rcases inv2 with ⟨ set2, countSet2, containsSet2⟩
+   have f1 := setMaxContainsBoth set1 set2
+   grind
+
+theorem learners_choice_is_unique (s : System a l p):
+ ∀ i j v1 v2, systemIsValid s -> (s.learners i).decide = some v1 -> (s.learners j).decide = some v2 -> v1 = v2 := by
+   intro i j v1 v2 sIsValid sDecV1 sDecV2
+   have t1 := decide_imp_set_exists s i v1 sIsValid
+   have t2 := decide_imp_set_exists s j v2  sIsValid
+   have f := set_inv_is_unique s v1 v2  i j
+   simp [systemIsValid, systemInits] at sIsValid;
+   have aBound: (a >= 2 ) := by (rcases sIsValid with ⟨ s0, rest⟩ ; simp [rest])
+   have f_ := f aBound
+   grind
