Distributed/paxos_proof4.lean
@@ -1,0 +1,113 @@
+import Distributed.base_structures
+import Distributed.paxos_model
+import Mathlib.Tactic.ByContra
+
+open Model
+open PaxosModel
+namespace PaxosProof
+
+
+def inv_1 (learners: Map l (Learner a l) ) (v: Value) (j: Fin l):=
+(learners j).decide = some v
+-> (∃  (s: Set a) (id: PropId), count s > a / 2 ∧  (∀ i, contains s i -> (learners j).decMap i = (v, id) )) 
+
+theorem inv1_holds (s1 s2: System a l p):
+∀ j v, step s1 s2 
+-> inv_1 s1.learners v j
+-> inv_1 s2.learners v j := by
+   intros j v step inv1
+   cases step <;> rename_i stepRule <;> cases stepRule <;> try grind
+   . rename_i i learner mess v' stepRule
+     simp [inv_1, updateMap] at *
+     split <;> try grind
+     intros decNone; have ⟨ x, rest ⟩ :=inv1 decNone
+     exists x 
+   . rename_i l1 v' i stepRule
+     simp [inv_1, updateMap] at *
+     split <;> try grind
+     rcases stepRule with ⟨ set, setCounts, setContains, setIsNone, set ⟩
+     intros l1Decs; exists set; simp [setCounts]; simp at l1Decs; subst l1Decs;
+     sorry
+     sorry
+     
+
+
+
+def inv_2 (learners: Map l (Learner a l)) (acceptors: Map a (Acceptor a) )  (j: Fin l) :=
+  ∀ i v (id: PropId), (learners j).decMap i = some (id, v) →
+    ∃ (id': PropId), id' ≥ id -> (acceptors i).accepted = some (id', v)
+
+theorem inv2_holds (s1 s2: System a l p):
+∀ j, step s1 s2 
+-> inv_2 s1.learners s1.acceptors  j
+-> inv_2 s2.learners s2.acceptors  j := by sorry
+
+
+def inv_3 (acceptors: Map a (Acceptor a) ) (v1 v2: Value) :=
+∀ (key1 key2: PropId),
+key1 <= key2
+-> (∃  (s: Set a), count s > a / 2 ∧  (∀ i, contains s i -> (acceptors i).accepted = some (key1, v1)))
+-> (∃  (s: Set a), count s > a / 2 ∧  (∀ i, contains s i -> (acceptors i).accepted = some (key2, v2)))
+-> v1 = v2
+
+theorem inv3_holds (s1 s2: System a l p):
+step s1 s2 
+-> inv_3  s1.acceptors v1 v2
+-> inv_3 s2.acceptors v1 v2 := by sorry
+
+
+
+/--     
+theorem inv2_holds (s1 s2: System a l p):
+∀ j v, step s1 s2 
+-> inv_2 s1.learners s1.acceptors v j
+-> inv_2 s2.learners s2.acceptors v j := by
+   intros j v s1Step IH
+   cases s1Step <;> rename_i stepRule <;> cases stepRule <;> try grind
+   . rename_i id i v' acc m stepRule
+     simp [inv_2] at *; intros set1 set1Counts set1Contains
+     rcases stepRule with ⟨ sAcc, sId, accNat ⟩ 
+     rcases (IH set1 set1Counts set1Contains) with ⟨ set2, set2Counts, set2Contains ⟩; subst_vars
+     have IHApp := IH set1 set1Counts set1Contains; 
+     rcases IHApp with ⟨set3,  set3Counts, set3Contains ⟩
+     simp [updateMap]; exists set3
+     simp [set3Counts]; intros i2 i2IsContained;
+     split <;> try grind
+     simp; sorry
+--/
+
+
+theorem inv_app (s : System a l p):
+ ∀ i v1 v2, systemIsValid s
+ -> inv_1 s.learners v1 i ∧ inv_2 s.learners s.acceptors i ∧ inv_3 s.acceptors v1 v2 := by
+   simp [systemIsValid]
+   intros i v1 v2 s0 inits sSteps
+   induction sSteps with
+   | refl =>
+     simp [systemInits, learnerInits, acceptorInits] at inits
+     simp [inv_1, inv_2, inv_3, inits]
+     sorry
+   | trans =>
+     rename_i s2 s3 Steps step IH
+     have c1 := inv1_holds s2 s3 i v1 step IH.left
+     have c2 := inv2_holds s2 s3 i  step IH.right.left
+     have c3 := inv3_holds s2 s3 step IH.right.right
+     grind
+
+
+
+
+
+theorem learners_choice_is_unique (s : System a l p):
+ ∀ i j v1 v2, systemIsValid s -> (s.learners i).decide = some v1 -> (s.learners j).decide = some v2 -> v1 = v2 := by
+   intros i j v1 v2 sIsValid sSomeV1 sSomeV2
+   have inv_true1 := inv_app s i v1 v2 sIsValid
+   have inv_true2 := inv_app s j v2 v1 sIsValid 
+   rcases inv_true1 with ⟨ i11, i12, i13 ⟩ 
+   rcases inv_true2 with ⟨ i21, i22, i23 ⟩
+   clear i23
+   simp [inv_1] at i11; simp [inv_1] at i21
+   have s1 := i11 sSomeV1; rcases s1 with ⟨set1, countsSet1, x1,containsSet1 ⟩; clear i11
+   have s2:= i21 sSomeV2; rcases s2 with ⟨set2, countsSet2, x2,containsSet2 ⟩ ; clear i21
+   simp [inv_2] at i12; simp [inv_2] at i22; simp [inv_3] at i13;
+   sorry
