Distributed/paxos_proof5.lean
@@ -1,0 +1,82 @@
+import Distributed.base_structures
+import Distributed.paxos_model
+import Mathlib.Tactic.ByContra
+
+open Model
+open PaxosModel
+namespace PaxosProof
+
+
+
+def set_invariant (s1 : System a l p) (v : Value) (learnerId : Fin l):=
+  ∃ (s : Set a), count s > a / 2 ∧
+    ∀ i, contains s i →
+      ∃ id, (s1.learners learnerId).decMap i = some (v, id)
+      ∧ (s1.acceptors i).accepted = some (v, id)
+
+
+theorem inv_proof_ (s1 s2: System a l p) (v: Value) (j: Fin l):
+step s1 s2 
+→ (s2.learners j).decide ≠ some v 
+→ (s1.learners j).decide ≠ some v := by
+   intros s1Step i IH
+   by_contra contra
+   cases s1Step <;> rename_i stepRule <;> cases stepRule <;> try grind
+   . rename_i i learn m v' x stepRule; simp at *
+     have ⟨ learnNat,mInNet, learnDec, iNat ⟩ := stepRule;clear stepRule; subst_vars
+     unfold updateMap at i; split at i <;> try grind
+   . rename_i l2 v' u pid stepRule; simp at *
+     have ⟨set, setCount, setContains, l2None, l2Nat ⟩ := stepRule
+     subst l2Nat; simp [updateMap] at i; split at i <;> try grind
+
+theorem inv_proof (s1 s2: System a l p) (v: Value):
+step s1 s2 
+→ (s1.learners j).decide = some v 
+→ (s2.learners j).decide = some v := by
+  intros step s1Dec
+  by_contra
+  have cc := inv_proof_ s1 s2 v
+  grind
+
+theorem set_inv_is_unique (s: System a l p) (i j: Fin l) (v1 v2: Value) : 
+set_invariant s v1 i 
+→ set_invariant s v2 j 
+→ v1 = v2 := by
+  intros setInv1 setInv2
+  simp [set_invariant] at *;
+  rcases setInv1 with ⟨ set1, countSet1, set1Contains ⟩
+  rcases setInv2 with ⟨ set2, countSet2, set2Contains ⟩ 
+  have f := setMaxContainsBoth set1 set2 countSet1 countSet2
+  rcases f with ⟨ k, icontainedSet1, icontainedSet2⟩
+  have ⟨ id1, eqV1⟩  := set1Contains k icontainedSet1
+  have ⟨ id2, eqV2⟩  := set2Contains k icontainedSet2
+  simp [eqV1] at eqV2
+  grind
+
+theorem decide_imp_set_invariant (s: System a l p) (j: Fin l) (v: Value) :
+systemIsValid s
+→ (s.learners j).decide = some v 
+→ set_invariant s v j  := by
+  simp [systemIsValid]; intros s0 s0Inits s0Steps sDecSome
+  induction s0Steps with
+  | refl =>
+    simp [systemInits, learnerInits] at s0Inits
+    simp [s0Inits, set_invariant]; exists fullSet; simp [fullSetCountsN a]
+    constructor <;> try grind
+  | trans s1 s2 s1Steps s1Step IH =>
+    cases s1Step <;> rename_i stepRule <;> cases stepRule <;> try (simp [set_invariant] at *<;>grind)
+    . sorry
+    . rename_i i learn m v' pid d stepRule; simp [updateMap, set_invariant] at *
+      split at sDecSome <;> try grind
+    . rename_i learn2 v' i pid stepRule
+      simp [updateMap, set_invariant, IH] at *
+      split at sDecSome <;> try grind
+      rename_i eq; subst eq; simp
+      grind
+    
+theorem learners_choice_is_unique (s : System a l p):
+ ∀ i j v1 v2, systemIsValid s -> (s.learners i).decide = some v1 -> (s.learners j).decide = some v2 -> v1 = v2 := by
+  intros i j v1 v2 sIsValid sDecSome1 sDecSome2
+  have h1 := decide_imp_set_invariant s i v1 sIsValid sDecSome1
+  have h2 := decide_imp_set_invariant s j v2 sIsValid sDecSome2
+  exact set_inv_is_unique s i j v1 v2 h1 h2
